bn_glob_p instead of bn_set_p (same for q, bp, bq)

proof/schnorr_protocol/leakage_freeness/Verify_CT.ec
@@ -2,11 +2,87 @@ require import List Int AllCore Distr.
 
 from Jasmin require import JModel.
 
-
 require import W64_SchnorrExtract_ct.
+require import BigNum_LF.
+require import ModularMultiplication_Concrete_CT.
+require import BarretReduction_Concrete_CT.
+require import MontomeryLadder_Concrete_CT.
 
-(* only makes sense if verify is not probabilitystic  *)
-lemma verify_ct : equiv [M(Syscall).verify ~ M(Syscall).verify : ={M.leakages} ==> ={M.leakages} ].
-proof.  proc. progress. inline*. sim. qed.
+(* verify LEAKAGES  *)
+op verify_f  : leakages_t =
+ LeakAddr [] :: bn_eq_t ++
+ LeakAddr [] :: set1_f 32 ++
+ LeakAddr [] :: expm_t ++
+ LeakAddr [] :: bn_eq_t ++
+ LeakAddr [] :: expm_t ++
+ LeakAddr [] :: mulm_t ++
+ LeakAddr [] :: expm_t ++
+ LeakAddr [] :: bn_breduce_small_f ++
+ LeakAddr [] :: bn_breduce_small_f ++
+ LeakAddr [] :: bn_breduce_small_f ++
+ LeakAddr [] :: bn_breduce_small_f ++
+ LeakAddr [] :: 
+ LeakAddr [] :: 
+ LeakAddr [] :: 
+ LeakAddr [] :: 
+ LeakAddr [] :: 
+ LeakAddr [] :: [].
+
+
+lemma verify_leakages start_l :
+   hoare [ M(Syscall).verify : M.leakages = start_l
+     ==> M.leakages = verify_f  ++ start_l ].
+proof. proc.
+wp. ecall (bn_eq_leakages M.leakages).
+wp. ecall (bn_set1_leakages M.leakages).
+wp. ecall (bn_expm_leakages M.leakages).
+wp. ecall (bn_eq_leakages M.leakages).
+wp. ecall (bn_expm_leakages M.leakages).
+wp. ecall (bn_mulm_leakages M.leakages).
+wp. ecall (bn_expm_leakages M.leakages).
+wp. ecall (bn_breduce_small_leakages M.leakages).
+wp. ecall (bn_breduce_small_leakages M.leakages).
+wp. ecall (bn_breduce_small_leakages M.leakages).
+wp. ecall (bn_breduce_small_leakages M.leakages).
+wp. skip. 
+progress.
+rewrite /verify_f.
+do ? (rewrite - catA; simplify).
+auto.
+qed.
+
+
+lemma verify_ll: islossless M(Syscall).verify.
+proc.
+wp. call (bn_eq_ll).
+wp. call (bn_set1_ll).
+wp. call (bn_expm_ll).
+wp. call (bn_eq_ll).
+wp. call (bn_expm_ll).
+wp. call (bn_mulm_ll).
+wp. call (bn_expm_ll).
+wp. call (bn_breduce_small_ll).
+wp. call (bn_breduce_small_ll).
+wp. call (bn_breduce_small_ll).
+wp. call (bn_breduce_small_ll).
+wp. auto.
+qed.
+
+
+lemma verify_leakages_ph start_l :
+   phoare [ M(Syscall).verify : M.leakages = start_l 
+     ==> M.leakages = verify_f  ++ start_l ] = 1%r.
+phoare split !  1%r 0%r. auto.
+conseq verify_ll. hoare. conseq (verify_leakages start_l).
+qed.
+
+
+lemma verify_ct &m l sin :  M.leakages{m} = l
+ => Pr[ M(Syscall).verify(sin)@&m : M.leakages = verify_f ++ l ] = 1%r.
+move => lh.
+byphoare (_: (glob M) = (glob M){m} ==> _ ).
+conseq (verify_leakages_ph l).
+auto. auto. auto.
+qed.
 
 
