proof/montgomery_ladder/leakage_freeness/MontomeryLadder_Concrete_CT.ec
@@ -57,7 +57,7 @@ qed.
 
 op [opaque] expm_t : leakages_t = expm_step 2048 ++ expm_t_prefix.
 
-lemma expm_leakages l :
+lemma bn_expm_leakages l :
   hoare [ M(Syscall).bn_expm : M.leakages = l
      ==> M.leakages = expm_t ++ l].
 proc.
@@ -94,11 +94,11 @@ wp.  call (bn_copy_leakages suf3).
 wp. skip. progress.
 pose suf4 :=  [LeakAddr []]  ++ copy_f 32 ++ suf3.
 seq 3 : (M.leakages = mulm_t ++ suf4 /\ i_var = i + W64.one /\ W64.zero \ult i_var /\ (i + W64.one <> W64.zero => i \ult (W64.of_int 2048))).
-wp.  call (mulm_leakages suf4).
+wp.  call (bn_mulm_leakages suf4).
 wp. skip. progress.
 pose suf5 :=  [LeakAddr []]  ++ mulm_t ++ suf4.
 seq 3 : (M.leakages = mulm_t ++ suf5 /\ i_var = i + W64.one /\ W64.zero \ult i_var /\ (i + W64.one <> W64.zero => i \ult (W64.of_int 2048))).
-wp.  call (mulm_leakages suf5).
+wp.  call (bn_mulm_leakages suf5).
 wp. skip. progress.
 pose suf6 :=  [LeakAddr []]  ++ mulm_t ++ suf5.
 seq 3 : (M.leakages = swapr_f 32 ++ suf6 /\ i_var = i + W64.one /\ W64.zero \ult i_var /\ (i + W64.one <> W64.zero => i \ult (W64.of_int 2048))).
@@ -159,7 +159,7 @@ lemma bn_expm_leakages_ph start_l :
    phoare [ M(Syscall).bn_expm : M.leakages = start_l
      ==> M.leakages = expm_t ++ start_l ] = 1%r.
 phoare split !  1%r 0%r. auto.
-conseq bn_expm_ll. hoare. conseq (expm_leakages start_l).
+conseq bn_expm_ll. hoare. conseq (bn_expm_leakages start_l).
 qed.
 
 lemma bn_expm_ct &m l r a b n :  M.leakages{m} = l
